src/HOL/IMP/Abs_Int1.thy
@@ -136,45 +136,45 @@ qed
 
 end
 
-fun top_on_st :: "vname set \<Rightarrow> 'a::top st \<Rightarrow> bool" where
-"top_on_st X F = (\<forall>x\<in>X. fun F x = \<top>)"
+fun top_on_st :: "'a::top st \<Rightarrow> vname set \<Rightarrow> bool" where
+"top_on_st S X = (\<forall>x\<in>X. fun S x = \<top>)"
 
-fun top_on_opt :: "vname set \<Rightarrow> 'a::top st option \<Rightarrow> bool" where
-"top_on_opt X (Some F) = top_on_st X F" |
-"top_on_opt X None = True"
+fun top_on_opt :: "'a::top st option \<Rightarrow> vname set \<Rightarrow> bool" where
+"top_on_opt (Some S)  X = top_on_st S X" |
+"top_on_opt None X = True"
 
-definition top_on_acom :: "vname set \<Rightarrow> 'a::top st option acom \<Rightarrow> bool" where
-"top_on_acom X C = (\<forall>a \<in> set(annos C). top_on_opt X a)"
+definition top_on_acom :: "'a::top st option acom \<Rightarrow> vname set \<Rightarrow> bool" where
+"top_on_acom C X = (\<forall>a \<in> set(annos C). top_on_opt a X)"
 
-lemma top_on_top: "top_on_opt X (\<top>::_ st option)"
+lemma top_on_top: "top_on_opt (\<top>::_ st option) X"
 by(auto simp: top_option_def fun_top)
 
-lemma top_on_bot: "top_on_acom X (bot c)"
+lemma top_on_bot: "top_on_acom (bot c) X"
 by(auto simp add: top_on_acom_def bot_def)
 
-lemma top_on_post: "top_on_acom X C \<Longrightarrow> top_on_opt X (post C)"
+lemma top_on_post: "top_on_acom C X \<Longrightarrow> top_on_opt (post C) X"
 by(simp add: top_on_acom_def post_in_annos)
 
 lemma top_on_acom_simps:
-  "top_on_acom X (SKIP {Q}) = top_on_opt X Q"
-  "top_on_acom X (x ::= e {Q}) = top_on_opt X Q"
-  "top_on_acom X (C1;C2) = (top_on_acom X C1 \<and> top_on_acom X C2)"
-  "top_on_acom X (IF b THEN {P1} C1 ELSE {P2} C2 {Q}) =
-   (top_on_opt X P1 \<and> top_on_acom X C1 \<and> top_on_opt X P2 \<and> top_on_acom X C2 \<and> top_on_opt X Q)"
-  "top_on_acom X ({I} WHILE b DO {P} C {Q}) =
-   (top_on_opt X I \<and> top_on_acom X C \<and> top_on_opt X P \<and> top_on_opt X Q)"
+  "top_on_acom (SKIP {Q}) X = top_on_opt Q X"
+  "top_on_acom (x ::= e {Q}) X = top_on_opt Q X"
+  "top_on_acom (C1;C2) X = (top_on_acom C1 X \<and> top_on_acom C2 X)"
+  "top_on_acom (IF b THEN {P1} C1 ELSE {P2} C2 {Q}) X =
+   (top_on_opt P1 X \<and> top_on_acom C1 X \<and> top_on_opt P2 X \<and> top_on_acom C2 X \<and> top_on_opt Q X)"
+  "top_on_acom ({I} WHILE b DO {P} C {Q}) X =
+   (top_on_opt I X \<and> top_on_acom C X \<and> top_on_opt P X \<and> top_on_opt Q X)"
 by(auto simp add: top_on_acom_def)
 
 lemma top_on_sup:
-  "top_on_opt X o1 \<Longrightarrow> top_on_opt X o2 \<Longrightarrow> top_on_opt X (o1 \<squnion> o2 :: _ st option)"
+  "top_on_opt o1 X \<Longrightarrow> top_on_opt o2 X \<Longrightarrow> top_on_opt (o1 \<squnion> o2 :: _ st option) X"
 apply(induction o1 o2 rule: sup_option.induct)
 apply(auto)
 by transfer simp
 
 lemma top_on_Step: fixes C :: "('a::semilattice)st option acom"
-assumes "!!x e S. \<lbrakk>top_on_opt X S; x \<notin> X; vars e \<subseteq> -X\<rbrakk> \<Longrightarrow> top_on_opt X (f x e S)"
-        "!!b S. top_on_opt X S \<Longrightarrow> vars b \<subseteq> -X \<Longrightarrow> top_on_opt X (g b S)"
-shows "\<lbrakk> vars C \<subseteq> -X; top_on_opt X S; top_on_acom X C \<rbrakk> \<Longrightarrow> top_on_acom X (Step f g S C)"
+assumes "!!x e S. \<lbrakk>top_on_opt S X; x \<notin> X; vars e \<subseteq> -X\<rbrakk> \<Longrightarrow> top_on_opt (f x e S) X"
+        "!!b S. top_on_opt S X \<Longrightarrow> vars b \<subseteq> -X \<Longrightarrow> top_on_opt (g b S) X"
+shows "\<lbrakk> vars C \<subseteq> -X; top_on_opt S X; top_on_acom C X \<rbrakk> \<Longrightarrow> top_on_acom (Step f g S C) X"
 proof(induction C arbitrary: S)
 qed (auto simp: top_on_acom_simps vars_acom_def top_on_post top_on_sup assms)
 
@@ -203,7 +203,7 @@ apply (transfer fixing: m)
 apply(simp add: less_eq_st_rep_iff eq_st_def m_s2_rep)
 done
 
-lemma m_o2: "finite X \<Longrightarrow> top_on_opt (-X) o1 \<Longrightarrow> top_on_opt (-X) o2 \<Longrightarrow>
+lemma m_o2: "finite X \<Longrightarrow> top_on_opt o1 (-X) \<Longrightarrow> top_on_opt o2 (-X) \<Longrightarrow>
   o1 < o2 \<Longrightarrow> m_o X o1 > m_o X o2"
 proof(induction o1 o2 rule: less_eq_option.induct)
   case 1 thus ?case by (auto simp: m_o_def m_s2 less_option_def)
@@ -213,25 +213,25 @@ next
   case 3 thus ?case by (auto simp: less_option_def)
 qed
 
-lemma m_o1: "finite X \<Longrightarrow> top_on_opt (-X) o1 \<Longrightarrow> top_on_opt (-X) o2 \<Longrightarrow>
+lemma m_o1: "finite X \<Longrightarrow> top_on_opt o1 (-X) \<Longrightarrow> top_on_opt o2 (-X) \<Longrightarrow>
   o1 \<le> o2 \<Longrightarrow> m_o X o1 \<ge> m_o X o2"
 by(auto simp: le_less m_o2)
 
 
-lemma m_c2: "top_on_acom (-vars C1) C1 \<Longrightarrow> top_on_acom (-vars C2) C2 \<Longrightarrow>
+lemma m_c2: "top_on_acom C1 (-vars C1) \<Longrightarrow> top_on_acom C2 (-vars C2) \<Longrightarrow>
   C1 < C2 \<Longrightarrow> m_c C1 > m_c C2"
 proof(auto simp add: le_iff_le_annos m_c_def size_annos_same[of C1 C2] vars_acom_def less_acom_def)
   let ?X = "vars(strip C2)"
-  assume top: "top_on_acom (- vars(strip C2)) C1"  "top_on_acom (- vars(strip C2)) C2"
+  assume top: "top_on_acom C1 (- vars(strip C2))"  "top_on_acom C2 (- vars(strip C2))"
   and strip_eq: "strip C1 = strip C2"
   and 0: "\<forall>i<size(annos C2). annos C1 ! i \<le> annos C2 ! i"
   hence 1: "\<forall>i<size(annos C2). m_o ?X (annos C1 ! i) \<ge> m_o ?X (annos C2 ! i)"
     apply (auto simp: all_set_conv_all_nth vars_acom_def top_on_acom_def)
     by (metis finite_cvars m_o1 size_annos_same2)
   fix i assume i: "i < size(annos C2)" "\<not> annos C2 ! i \<le> annos C1 ! i"
-  have topo1: "top_on_opt (- ?X) (annos C1 ! i)"
+  have topo1: "top_on_opt (annos C1 ! i) (- ?X)"
     using i(1) top(1) by(simp add: top_on_acom_def size_annos_same[OF strip_eq])
-  have topo2: "top_on_opt (- ?X) (annos C2 ! i)"
+  have topo2: "top_on_opt (annos C2 ! i) (- ?X)"
     using i(1) top(2) by(simp add: top_on_acom_def size_annos_same[OF strip_eq])
   from i have "m_o ?X (annos C1 ! i) > m_o ?X (annos C2 ! i)" (is "?P i")
     by (metis 0 less_option_def m_o2[OF finite_cvars topo1] topo2)
@@ -249,16 +249,16 @@ locale Abs_Int_measure =
   for \<gamma> :: "'av::semilattice \<Rightarrow> val set" and m :: "'av \<Rightarrow> nat"
 begin
 
-lemma top_on_step': "\<lbrakk> vars C \<subseteq> -X; top_on_acom X C \<rbrakk> \<Longrightarrow> top_on_acom X (step' \<top> C)"
+lemma top_on_step': "\<lbrakk> top_on_acom C (-vars C) \<rbrakk> \<Longrightarrow> top_on_acom (step' \<top> C) (-vars C)"
 unfolding step'_def
 by(rule top_on_Step)
   (auto simp add: top_option_def fun_top split: option.splits)
 
 lemma AI_Some_measure: "\<exists>C. AI c = Some C"
 unfolding AI_def
-apply(rule pfp_termination[where I = "\<lambda>C. strip C = c \<and> top_on_acom (- vars C) C" and m="m_c"])
+apply(rule pfp_termination[where I = "\<lambda>C. top_on_acom C (- vars C)" and m="m_c"])
 apply(simp_all add: m_c2 mono_step'_top bot_least top_on_bot)
-apply(auto simp add: top_on_step' vars_acom_def)
+using top_on_step' apply(auto simp add: vars_acom_def)
 done
 
 end
